src/sys_verif/program_proof/persistently.v
@@ -1,0 +1,334 @@
+(*| # Lecture 13: The persistently modality
+
+> Follow these notes in Coq at [src/sys_verif/program_proof/persistently.v](https://github.com/tchajed/sys-verif-fa24-proofs/blob/main/src/sys_verif/program_proof/persistently.v).
+
+## Learning outcomes
+
+- Read IPM goals with spatial and persistent contexts.
+- Explain the difference between top-level specifications and Hoare triples in separation logic.
+
+## Motivation
+
+We know that separation logic propositions are generally not duplicable ($P \nvdash P \sep P$). This is because we interpret propositions as asserting exclusive ownership, for example over heap locations. However, ownership does not _have_ to be exclusive. We've already seen one example with pure propositions $\lift{\phi}$, which can be freely duplicated and in the IPM even moved out of the spatial context into the Coq context. Another example where ownership isn't exlusive is if a pointer is _read-only_, it is safe to have many copies of its points-to fact, as long as those assertions are used only for reading and not writing.
+
+Before getting into modalities, let's revisit the mechanisms in Coq for read-only pointers.
+
+|*)
+
+From sys_verif.program_proof Require Import prelude empty_ffi.
+From Goose.sys_verif_code Require Import memoize.
+
+Section proof.
+Context `{hG: !heapGS Σ}.
+
+(*| ## Read-only pointers
+
+We saw in a previous lecture, and in the [fractions guide](/notes/program-proofs/fractions.md), how _fractional permissions_ can be used for read-only access.
+
+Recall the basic splitting/recombining rule:
+
+$l ↦_{q_1 + q_2} v ⊣⊢ l ↦_{q_1} v ∗ l ↦_{q_2} v$
+
+We can see splitting at work in this example, which first splits the assertion `l ↦[uint64T] #x` (using `iDestruct`, which knows to split a fractional points-to into two halves), then uses the two halves for the two loads.
+
+Fractions also support _combining_ to recover full ownership and go back to being able to write to the pointer.
+
+|*)
+
+Lemma split_fraction_example (l: loc) (x: w64) :
+  {{{ l ↦[uint64T] #x ∗ ⌜uint.Z x < 100⌝ }}}
+    let: "y" := ![uint64T] #l in
+    let: "z" := ![uint64T] #l in
+    #l <-[uint64T] ("y" + "z")
+  {{{ RET #(); l ↦[uint64T] #(LitInt (word.add x x)) }}}.
+Proof.
+  wp_start as "H".
+  iDestruct "H" as "[Hx %Hbound]".
+  iDestruct "Hx" as "[Hx1 Hx2]".
+  wp_apply (wp_LoadAt with "[$Hx1]"). iIntros "Hx1".
+  wp_apply (wp_LoadAt with "[$Hx2]"). iIntros "Hx2".
+  iCombine "Hx1 Hx2" as "Hx".
+  wp_store.
+  iModIntro.
+  iApply "HΦ".
+  iFrame.
+Qed.
+
+(*| ## Persistent propositions
+
+Fractions are good but don't directly give something duplicable. The _persistent points-to_ will solve this problem.
+
+Persistent propositions are a core feature of Iris. They are important enough that the Iris Proof Mode has a separate _persistent context_; so far it has been empty so we haven't seen it. The persistent context is separate from the _spatial context_. The persistent context contains only persistent resources, which are duplicable, but they are not pure, so they can talk about the heap memory for example. When we split a proof with `iSplitL` or when using `iApply` the persistent context will always be available in all subgoals; the assertions are implicitly duplicated by the proof mode when splitting.
+
+The IPM goals in general look like the following:
+
+```txt title="IPM goal"
+P, Q: iProp Σ
+------------
+"HP": P
+----------□
+"HQ": Q
+----------∗
+R
+```
+
+As usual, there is a Coq context above everything. The separation logic part has separation logic hypotheses "HP" and "HQ", and separation logic conclusion R. The fact that "HP" is in the persistent context implies that P is persistent - this means $P ⊢ P ∗ P$. (The full definition is more than that, but we won't go deep enough into how Iris works to talk about it.)
+
+So what propositions are persistent? First, the pure propositions are persistent - but they can be put into the Coq context, so they aren't so interesting. The first "real" example we'll see is the persistent points-to, `l ↦□ v`.
+
+|*)
+
+Lemma alloc_ro_spec (x: w64) :
+  {{{ True }}}
+    ref_to uint64T #x
+  {{{ (l: loc), RET (#l: val); l ↦[uint64T]□ #x }}}.
+Proof.
+  iIntros (Φ) "_ HΦ".
+  rewrite -wp_fupd.
+  wp_alloc l as "H".
+  (*| This is the step where we persist the points-to permission and turn it
+  into a persistent, read-only fact. Using `struct_pointsto_persist` requires the `iMod` tactic, which we will cover later when we talk about concurrency; for now think of it as a variation on `iDestruct`. |*)
+
+  iMod (struct_pointsto_persist with "H") as "#Hro".
+  (*| Notice from the goal diff that the output (renamed to "Hro" for clarity)
+is put into a separate list of hypotheses - this is the persistent context.
+
+To obtain the persistent points-to assertion, we have to give up the regular fractional assertion, and this operation is _not_ reversible - the persistence relies on the location never being written to. |*)
+  iModIntro.
+  iApply "HΦ".
+  iFrame "Hro".
+Qed.
+
+(*| With a persistent permission, it's reasonable (and expected) that the
+permission need not be returned in the postcondition. |*)
+Lemma read_discarded_spec (l: loc) (x: w64) :
+  {{{ l ↦[uint64T]□ #x }}}
+    ![uint64T] #l
+  {{{ RET #x; True }}}.
+Proof.
+  wp_start as "#H".
+  wp_apply (wp_LoadAt with "H"). iIntros "_".
+  iApply "HΦ". auto.
+Qed.
+
+(*| ### Exercise: why not return the points-to?
+
+When an assertion is persistent, we don't need to return it in the postcondition. Why?
+|*)
+
+(*| ## The persistently modality |*)
+
+(*| Motivated by this kind of shared ownership, we introduce a modality called the "persistently" modality, written $□P$. When $P$ is a proposition, $□P$ is another proposition which asserts that $P$ holds but without exclusive ownership.
+
+The main fact about persistently is that it is automatically duplicable: $□P ⊢ □P ∗ P$. It is also the case that $□P ∗ P ⊢ □P$. So $□P$ behaves a bit like $\lift{\phi}$ so far - if we prove it, it will remain true and not get "used up" in a proof.
+
+The general idea of a modality in logic is that it is a _shade of truth_ of another proposition. This can be a confusing concept, so we will approach it in several different ways. On first read, you need not understand the rest of this section; it might help to start by seeing it used in proofs in Coq before going back to the theory. We'll also be able to be more precise when we talk about concurrency.
+
+To understand the explanations of persistently it helps to anticipate a little of what we will talk about when introducing ghost state to reason about concurrent programs. Thus far, we said separation logic propositions have been predicates over the heap. We will extend this to be predicates over _resources_, where individual heap locations will be just one example. In fact we've already seen that the fractional permission $\ell ↦_{1/2} v$ can't be explained as a predicate over the heap (what do we do with the $1/2$ part? what does separation mean?). We will have to leave the notion of a "resource" abstract for now, but we will have regular exclusive resources, and persistent resources. $□P$ means $P$ holds over only the persistent resources. For now, you can imagine that we divide the heap into a two parts $(h_r, h_w)$ where $h_r$ is read-only. The read-only part turns out to be duplicable, in that we can consider $h_r$ and $h_r$ to be separate for proving $P ∗ Q$; there's no conflict between them since the values in that part of the heap don't change. On the other hand if $P$ and $Q$ mention exclusive resources (locations in $h_w$), then for $P ∗ Q$ to be true in a heap those read-write locations would have to be disjoint.
+
+
+First, it is useful to ask whether $□P$ is stronger or weaker than $P$ (in general a modality could be neither, but the modalities in Iris are one or the other). In this case, the answer is that it is _stronger_: $□P ⊢ P$ but not vice versa (in general). Intuitively, it's because $□P$ requires $P$ hold using only "persistent resources".
+
+Second, the persistence modality is monotonic - if $P ⊢ Q$, then $□P ⊢ □Q$. I think in some ways this is a basic sanity test of a modality, but I am not sure about this in general.
+
+Third, since $□P$ is $P$ using only persistent resources, $□P ⊢ □□P$; both sides don't use resources, and saying it twice makes no difference.
+
+### Exercise: introduction rule
+
+Prove this derived rule:
+
+$$
+\dfrac{□P ⊢ Q}{□P ⊢ □Q} \eqnlabel{persistently-intro}
+$$
+
+Fourth, a core feature of persistence is this rule:
+
+$$
+\dfrac{S ⊢ □P ∧ Q}%
+{S ⊢ □P ∗ Q} \eqnlabel{persistently-sep}
+$$
+
+This is more complicated than the other properties. We won't go into too much detail on this one, since it requires a little more understanding of resources than we have right now.
+
+Finally, we will introduce a notion of a "persistent proposition". Define `Persistent P` to be true if $P ⊢ □P$. For example, $ℓ ↦□ v$ is persistent.
+
+Don't get confused between $P$ being persistent and $□P$ ("persistently $P$")! If $P$ is persistent, observe that adding the modality in front makes no difference - $P ⊣⊢ □P$ from the rules above. On the other hand we can write $□Q$ for any $Q$, whether it's persistent or not.
+
+### Exercise: test your intuition about persistently
+
+What do you think $□(ℓ ↦ v)$ means?
+
+---
+
+|*)
+
+(*| ## Memoization example |*)
+
+(*| A core use of persistence is in Hoare triples, when they are used _within the logic_; that is, when we need to refer to the specification of a function within a proposition. The natural place this comes up is whenever a function is a value in our code, either as a parameter or as a struct field. We'll now introduce an extended example on memoization to introduce this.
+
+You should start by quickly reading the code for this example at [go/memoize/memoize.go](https://github.com/tchajed/sys-verif-fa24-proofs/blob/main/go/memoize/memoize.go).
+
+|*)
+
+
+(*| ### MockMemoize proof
+
+As a warmup, we'll verify the "MockMemoize" implementation. This version still has to store and call the function, but there's no memoization happening - when we use `m.Call(x)` it just always calls `f(x)`.
+
+There is another difference between the two implementations: we use a `*MockMemoize` whereas we'll use `Memoize` - one is always used through a pointer, while the other is used as a value. Both would work in this case, we're just illustrating what this looks like in the proofs.
+
+---
+
+To give a specification to the memoization library, we will require that the user prove that the provided function, which we'll call `f_body` (of type `val`, since it's a function in GooseLang), implements a Gallina function `f : w64 → w64`. This is more restrictive than strictly necessary, but we do need it to have some Hoare triple, since it must at minimum be safe to call, and if we want to say anything about the result of `Call` we also need to know what it does. The choice here is to require it to implement some pure function over integers, but which is one is arbitrary.
+
+The core of the proof is the representation invariant for a `*MockMemoize`. The most interesting part of that invariant is how we say that `f_body` implements `f: w64 → w64`.
+
+|*)
+
+Definition fun_implements (f_body: val) (f: w64 → w64) : iProp Σ :=
+  ∀ (x:w64), {{{ True }}} f_body #x {{{ RET #(f x); True }}}.
+
+#[export] Instance fun_implements_persistent f_body f :
+  Persistent (fun_implements f_body f).
+Proof. apply _. Qed.
+
+(*| 
+`fun_implements` is different from what you've seen so far in this class because it states the correctness of `f_body` as an `iProp` rather than a `Prop`. This is significant later, when we'll use `fun_implements` inside a precondition.
+
+The way this works is that a Hoare triple $\hoare{P}{e}{Q}$ when used as an iProp actually expands to:
+
+$$□(P \wand \wp(e, Q))$$
+
+### Exercise: what does persistently of a wand mean?
+
+Try to puzzle out what it means to prove this persistently vs not. You might want to come back to this after seeing the memoization proof (even for the mock memoization library) and where `fun_implements` is used.
+
+---
+
+|*)
+
+(*| There are several interesting things in the representation function `own_mock_memoize` below:
+
+- The `□` in `m ↦[MockMemoize :: "f"]□ f_body` makes this a persistent, read-only field points-to fact.
+- The names "#Hf" and "#Hf_spec" have a # which means they will be added to the
+  Iris Proof Mode's persistent context when introduced.
+
+|*)
+
+Definition own_mock_memoize (m: loc) (f: w64 → w64) : iProp Σ :=
+   ∃ (f_body: val),
+     "#Hf" :: m ↦[MockMemoize :: "f"]□ f_body ∗
+     "#Hf_spec" :: fun_implements f_body f.
+
+Lemma wp_NewMockMemoize (f_body: val) (f: w64 → w64) :
+  (* NOTE: this val_ty is an unnecessary restriction in Goose *)
+  val_ty f_body (arrowT uint64T uint64T) →
+  {{{ fun_implements f_body f }}}
+    NewMockMemoize f_body
+  {{{ l, RET #l; own_mock_memoize l f }}}.
+Proof.
+  intros Hty.
+  wp_start as "#Hf".
+  wp_pures.
+  (* NOTE: [wp_apply] will lose the |==> (update) modality here, but we can add
+  it ourselves with this rewrite. *)
+  rewrite -wp_fupd.
+  wp_alloc m as "Hm".
+  iApply struct_fields_split in "Hm". iNamed "Hm".
+  iMod (struct_field_pointsto_persist with "f") as "#f".
+  (*| The use of `iMod` above has turned our regular points-to (for a struct
+  field) into a persistent fact. We can never write to that field again in the
+  proof, but in exchange the assertion is persistent. |*)
+  iModIntro. iApply "HΦ".
+  (* `iFrame` doesn't use the persistent context by default (for performance
+  reasons primarily), but we can ask it to by passing `#` as an argument. *)
+  iFrame "#".
+Qed.
+
+(*| Once an `own_mock_memoize` is set up, using it is very straightforward. |*)
+Lemma wp_MockMemoize__Call l f (x0: w64) :
+  {{{ own_mock_memoize l f }}}
+    MockMemoize__Call #l #x0
+  {{{ RET #(f x0); True }}}.
+Proof.
+  wp_start as "#Hm". iNamed "Hm".
+  wp_pures.
+  wp_loadField.
+  (*| Observe how in the next line we use a Hoare triple that comes _from the persistent_ context. The correctness of `f` isn't coming from a Coq lemma, but from within separation logic.
+
+   (Unfolding `fun_implements` isn't required, it's only there to show you the definition in the goal.)
+|*)
+  rewrite /fun_implements. wp_apply "Hf_spec".
+  iApply "HΦ". done.
+Qed.
+
+(*| ### Memoize proof
+
+Now we'll provide the same interface, but with actual memoization.
+
+|*)
+
+Definition own_memoize (m: val) (f: w64 → w64) : iProp Σ :=
+   ∃ (f_body: val) (m_ref: loc) (results: gmap w64 w64),
+     (* Notice that the map is modeled as a location. This reflects how Go maps
+     work (the value of that pointer does not change as you update the map). *)
+     "%Hmeq" :: ⌜m = (f_body, (#m_ref, #()))%V⌝ ∗
+     "#Hf_spec" :: fun_implements f_body f ∗
+     "Hm" :: own_map m_ref (DfracOwn 1) results ∗
+     (* This is the invariant that gives the correctness of the
+     memoization. *)
+     "%Hresults" :: ⌜∀ x y, results !! x = Some y → y = f x⌝.
+
+Lemma wp_NewMemoize (f_body: val) (f: w64 → w64) :
+  {{{ fun_implements f_body f }}}
+    NewMemoize f_body
+  {{{ v, RET v; own_memoize v f }}}.
+Proof.
+  wp_start as "#Hf".
+  wp_apply (wp_NewMap w64). iIntros (m_ref) "Hm".
+  wp_pures.
+  iModIntro. iApply "HΦ".
+  iFrame "Hf Hm".
+  iPureIntro.
+  split; auto.
+  intros x y Hget. rewrite lookup_empty in Hget.
+  congruence.
+Qed.
+
+Lemma wp_Memoize__Call v f (x0: w64) :
+  {{{ own_memoize v f }}}
+    Memoize__Call v #x0
+  {{{ RET #(f x0); own_memoize v f }}}.
+Proof.
+  wp_start as "Hm".
+  iNamed "Hm". subst.
+  wp_pures.
+  wp_apply (wp_MapGet with "Hm"). iIntros (v ok) "[%Hmap_get Hm]".
+  wp_pures.
+  wp_if_destruct; subst.
+  - apply map_get_true in Hmap_get.
+    iModIntro.
+    replace v with (f x0).
+    { iApply "HΦ". iFrame "#∗". eauto. }
+    apply Hresults in Hmap_get; auto.
+  - wp_pures.
+    wp_apply "Hf_spec". wp_pures.
+    wp_apply (wp_MapInsert with "Hm").
+    { auto. }
+    iIntros "Hm".
+    rewrite /map_insert.
+    wp_pures.
+    iModIntro.
+    iApply "HΦ".
+    iFrame "#∗".
+    iSplit; [ eauto | ].
+    iPureIntro.
+    intros x y.
+    intros Hget.
+    destruct (decide (x0 = x)); subst.
+    { rewrite lookup_insert in Hget. congruence. }
+    rewrite lookup_insert_ne // in Hget.
+    eauto.
+Qed.
+
+End proof.
